src/utils/stream.v
@@ -1,3 +1,0 @@
-CoInductive stream : Set :=
-| Cons (h: nat) (t: stream)
-| Nil.
